src/Appraisal_AltImpls_Eq.v
@@ -101,6 +101,7 @@ Proof.
     }
     subst.
     repeat ff.
+    jkjke.
   -
     ff.
     assert (exists et1 et2, et = ss et1 et2).
