src/Test_Extract_App.v
@@ -1,8 +1,10 @@
 Require Extraction.
 
-Require Import Impl_appraisal.
+Require Import Impl_vm Impl_appraisal_alt.
 
 Extraction Language CakeML.
+
+Recursive Extraction copland_compile.
 
 
 Recursive Extraction build_app_comp_evC.
